src/Init/Data/List/MinMax.lean
@@ -218,7 +218,7 @@ theorem min_eq_headV {α : Type u} [Min α] {l : List α} (hl : l ≠ [])
     (h : l.Pairwise (fun a b => min a b = a)) :
     haveI : Nonempty α := ⟨l.head hl⟩
     l.min hl = l.headV := by
-  simp [min_eq_head hl h, head_eq_headV hl]
+  simp [min_eq_head hl h]
 
 @[grind .]
 theorem min_mem [Min α] [MinEqOr α] {l : List α} (hl : l ≠ []) : l.min hl ∈ l :=
@@ -447,7 +447,7 @@ theorem max_eq_headV {α : Type u} [Max α] {l : List α} (hl : l ≠ [])
     (h : l.Pairwise (fun a b => max a b = a)) :
     haveI : Nonempty α := ⟨l.head hl⟩
     l.max hl = l.headV := by
-  simp [max_eq_head hl h, head_eq_headV hl]
+  simp [max_eq_head hl h]
 
 @[grind .]
 theorem max_mem [Max α] [MaxEqOr α] {l : List α} (hl : l ≠ []) : l.max hl ∈ l :=
