src/Std/Data/DHashMap/Lemmas.lean
@@ -5665,13 +5665,13 @@ theorem isEmpty_filter_eq_false_iff [LawfulBEq α]
 theorem isEmpty_filter_key_iff [EquivBEq α] [LawfulHashable α]
     {f : α → Bool} :
     (m.filter (fun a _ => f a)).isEmpty ↔
-      ∀ (k : α) (_ : k ∈ m), f (m.getKeyV k) = false :=
+      ∀ (k : α), k ∈ m → f (m.getKeyV k) = false :=
   Raw₀.isEmpty_filter_key_iff ⟨m.1, _⟩ m.2
 
 theorem isEmpty_filter_key_eq_false_iff [EquivBEq α] [LawfulHashable α]
     {f : α → Bool} :
     (m.filter (fun a _ => f a)).isEmpty = false ↔
-      ∃ (k : α) (_ : k ∈ m), f (m.getKeyV k) :=
+      ∃ (k : α), k ∈ m ∧ f (m.getKeyV k) :=
   Raw₀.isEmpty_filter_key_eq_false_iff ⟨m.1, _⟩ m.2
 
 @[grind =, cbv_eval]
@@ -5742,7 +5742,7 @@ theorem filter_key_equiv_self_iff [EquivBEq α] [LawfulHashable α]
 
 theorem size_filter_key_eq_size_iff [EquivBEq α] [LawfulHashable α]
     {f : α → Bool} :
-    (m.filter fun k _ => f k).size = m.size ↔ ∀ (k : α) (_ : k ∈ m), f (m.getKeyV k) :=
+    (m.filter fun k _ => f k).size = m.size ↔ ∀ (k : α), k ∈ m → f (m.getKeyV k) :=
   Raw₀.size_filter_key_eq_size_iff ⟨m.1, _⟩ m.2
 
 @[simp, grind =, cbv_eval]
