src/Std/Data/HashSet/Raw.lean
@@ -164,6 +164,10 @@ If no panic occurs the result is guaranteed to be pointer equal to the key in th
 @[inline] def get! [BEq α] [Hashable α] [Inhabited α] (m : Raw α) (a : α) : α :=
   m.inner.getKey! a
 
+/--
+Checks if given key is contained and returns the key if it is, otherwise returns `Classical.ofNonempty`.
+If the key is contained the result is guaranteed to be pointer equal to the key in the set.
+-/
 noncomputable def getV [BEq α] [Hashable α] (m : Raw α) (a : α) : α :=
   haveI : Nonempty α := ⟨a⟩
   m.getD a Classical.ofNonempty
