src/Std/Data/TreeSet/Raw/Lemmas.lean
@@ -2500,14 +2500,15 @@ theorem toArray_filter {f : α → Bool} (h : t.WF) :
 @[grind =] theorem isEmpty_filter_iff [TransCmp cmp]
     {f : α → Bool} (h : t.WF) :
     (t.filter f).isEmpty ↔
-      ∀ (k : α) (_ : k ∈ t), f (t.getV k) = false :=
+      ∀ (k : α), k ∈ t → f (t.getV k) = false :=
   TreeMap.Raw.isEmpty_filter_iff h.out
 
 theorem isEmpty_filter_eq_false_iff [TransCmp cmp]
     {f : α → Bool} (h : t.WF) :
     (t.filter f).isEmpty = false ↔
-      ∃ (k : α) (_ : k ∈ t), f (t.getV k) :=
-  TreeMap.Raw.isEmpty_filter_eq_false_iff h.out
+      ∃ (k : α), k ∈ t ∧ f (t.getV k) := by
+  rw [← Bool.not_eq_true, isEmpty_filter_iff h]
+  simp only [Classical.not_forall, Bool.not_eq_false, exists_prop]
 
 -- TODO: `contains_filter` is missing.
 
@@ -2515,8 +2516,8 @@ theorem isEmpty_filter_eq_false_iff [TransCmp cmp]
 theorem mem_filter [TransCmp cmp]
     {f : α → Bool} {k : α} (h : t.WF) :
     haveI : Nonempty α := ⟨k⟩
-    (k ∈ t.filter f) ↔ ∃ (_ : k ∈ t), f (t.getV k) :=
-  TreeMap.Raw.mem_filter h.out
+    (k ∈ t.filter f) ↔ k ∈ t ∧ f (t.getV k) :=
+  (TreeMap.Raw.mem_filter h.out).trans exists_prop
 
 theorem mem_filter_iff_get [TransCmp cmp]
     {f : α → Bool} {k : α} (h : t.WF) :
@@ -2537,7 +2538,7 @@ grind_pattern size_filter_le_size => (t.filter f).size
 
 theorem size_filter_eq_size_iff [TransCmp cmp]
     {f : α → Bool} (h : t.WF) :
-    (t.filter f).size = t.size ↔ ∀ (k : α) (_ : k ∈ t), f (t.getV k) :=
+    (t.filter f).size = t.size ↔ ∀ (k : α), k ∈ t → f (t.getV k) :=
   TreeMap.Raw.size_filter_eq_size_iff h.out
 
 theorem filter_equiv_self_iff [TransCmp cmp]
